verification_finalised/bank/spares.dfy
@@ -1,0 +1,18 @@
+// Remove unit from the system, this function requires the unit 
+// to be in the system since it does not make sense to remove a unit 
+// which is not there. This function does not preserve the order of the list.
+method RemoveUnit(unit: int)
+requires unit in units;
+ensures |units| == |old(units)| - 1;
+ensures forall i :: (0<=i<|old(units)| && old(units[i]) != unit) ==> old(units[i]) in units; 
+{
+    var key := FindUnitIndex(unit);
+    units := units[..key] + units[(key+1)..];
+}
+
+// Test 1: 
+bank := new BloodBank();
+bank.AddUnit(1); assert 1 in bank.units;
+bank.AddUnit(2); assert 2 in bank.units;
+bank.RemoveUnit(1); assert 1 !in bank.units; assert 2 in bank.units;
+i2 := bank.FindUnitIndex(2); assert i2 == 0;
